---
title: "Proofs"
output:
  pdf_document:
    latex_engine: xelatex
---

Consider data for variable x = $x_1$, $x_2$, . . . , $x_n$. We use x to denote the sample mean of x, and $s_x$ is the sample standard deviation of x.

# Part I

For each of the following three transformations derive (a) the sample mean z, and (b) the sample standard
deviation $s_z$.

1. Centering

$z_i$ = ($x_i$ − x)

$$
\def\zbar{\overline{z}}
\def\sumn{\sum_{i=1}^{n}}
\def\xbar{\overline{x}}


\zbar = \frac{1}{n}\sum(z_i)\\
= \frac{1}{n}\sum(x_i-\xbar)\\
= \frac{1}{n}\sum(x_i)-\frac{1}{n}\sum(\xbar)\\
=\xbar-\xbar\\
=0\\

S_z^2=\frac{1}{n}\sum(z_i-\zbar)\\
=\frac{1}{n}\sum(z_i-0)^2\\
=\frac{1}{n}\sum(z_i)^2\\
=\frac{1}{n}\sum(x_i-\xbar)^2\\
=\sigma^2(x)\\

S_z=\sqrt(S_z^2)\\
=\sqrt(\sigma^2(x))\\
=\sigma(x)
$$
2. Scaling
$$
z_i = \frac{x_i}{S_x}\\
\\
\zbar=\frac{1}{n}\sum(z_i)\\
=\frac{1}{n}\sum(\frac{x_i}{S_x})\\
=\frac{1}{n}\frac{1}{S_x}\sum(x_i)\\
=\frac{\xbar}{S_x}\\

S_z^2=\frac{1}{n}\sum(z_i-\zbar)^2\\
=\frac{1}{n}\sum(\frac{x_i}{S_x}-\frac{\xbar}{S_x})^2\\
=\frac{1}{n}\sum(\frac{x_i^2}{S_x^2}-\frac{2x_i\xbar}{S_x^2}+\frac{\xbar^2}{s_x^2})\\
=\frac{1}{S_x^2}\frac{1}{n}\sum(x_i^2-2x_i\xbar+\xbar^2)\\
=\frac{1}{S_x^2}\frac{1}{n}\sum(x_i-\xbar)^2\\
=\frac{1}{S_x^2}S_x^2\\
=1\\

S_z=\sqrt(S_z^2)=1
$$
3. Centering and scaling (standardizing)
$$
z_i = \frac{(x_i − x)}{S_x}
$$
$$
\zbar=\frac{1}{n}\sum(z_i)\\
=\frac{1}{n}\sum(\frac{x_i-\xbar}{S_x})\\
=\frac{1}{n}\frac{1}{S_x}\sum(x_i-\xbar)\\
=\frac{1}{S_x}\frac{1}{n}[\sum(x_i)-\sum(\xbar)]\\
=\frac{1}{S_x}[\frac{1}{n}\sum(x_i)-\frac{1}{n}\sum(\xbar)]\\
=\frac{1}{S_x}(\xbar-\xbar)\\
=\frac{1}{S_x}(0)\\
=0\\

\S_z^2=\frac{1}{n}\sum(z_i)^2\\
=\frac{1}{n}\sum(\frac{x_i-\xbar}{S_x})^2\\
=\frac{1}{S_x}\frac{1}{n}\sum(x_i-\xbar)^2\\
=\frac{1}{S_x}S_x^2\\
=1\\

S_z=\sqrt{S_z^2}=1
$$

# Part II
4. Consider transformation $z_i$ = $\log(x_i)$. 
Show that the sample mean $\zbar$ equals the logarithm of the
geometric sample mean of the original data $x_i$.

Note: The sample mean we use most commonly is the arithmetic mean (x = $\frac{1}{n}\sum(x_i)$. For strictly positive data, especially where there is skew, the geometric mean is a better summary of central trend. It is defined as:
gm(x) = $(\prod_{i=1}^nx_i)^\frac{1}{n}$
So, your problem is to show that $\zbar = \log(gm(x))$.

$$

\zbar=\frac{1}{n}\sum(z_i)\\
=\frac{1}{n}\sum(\log(x_i))\\
=\frac{1}{n}(\log(x_1)+\log(x_2)+...)\\
=\log(x_1)^\frac{1}{n}+\log(x_2)^\frac{1}{n}+...\\
=\log(x_1^\frac{1}{n}*x_2^\frac{1}{n}*x_3^\frac{1}{n}...)\\
=\log(\prod(x_i)^\frac{1}{n})\\
=\log(gm(x))

$$

